books/centaur/fgl/nat-var-aig.lisp
@@ -36,49 +36,117 @@
 (include-book "centaur/aig/aig-vars" :dir :system)
 (include-book "centaur/misc/fast-alist-pop" :dir :system)
 (include-book "std/stobjs/absstobjs" :dir :system)
+(local (include-book "std/basic/arith-equivs" :dir :system))
 
-(std::deflist nat-listp (x) (natp x) :already-definedp t :true-listp t :elementp-of-nil nil)
+(local (std::add-default-post-define-hook :fix))
 
-(define aig-p (x)
+(define bounded-natp (x (bound natp))
+  (and (natp x)
+       (< x (nfix bound)))
+  ///
+  (defthm bounded-natp-implies-bound
+    (implies (bounded-natp x bound)
+             (< x (nfix bound)))
+    :rule-classes :forward-chaining)
+
+  (defthm bounded-natp-implies-natp
+    (implies (bounded-natp x bound)
+             (natp x))
+    :rule-classes :forward-chaining)
+
+  (defthm bounded-natp-of-nil
+    (not (bounded-natp nil bound)))
+
+  (defthm bounded-natp-when-bounded-by-less
+    (implies (and (bounded-natp x bound1)
+                  (<= (nfix bound1) (nfix bound)))
+             (bounded-natp x bound))))
+
+(define bounded-nat-listp (x (bound natp))
+  (if (atom x)
+      t
+    (and (bounded-natp (car x) bound)
+         (bounded-nat-listp (cdr x) bound)))
+  ///
+  (defthm bounded-nat-listp-when-bounded-by-lesser
+    (implies (and (bounded-nat-listp x bound1)
+                  (<= (nfix bound1) (nfix bound)))
+             (bounded-nat-listp x bound)))
+
+  (defthmd not-bounded-nat-listp-by-member
+    (implies (and (member k x)
+                  (not (bounded-natp k bound)))
+             (not (bounded-nat-listp x bound))))
+
+  (defthmd bounded-nat-listp-implies-not-member
+    (implies (and (bounded-nat-listp x bound)
+                  (not (bounded-natp k bound)))
+             (not (member k x))))
+
+  (defthm bounded-nat-listp-of-append
+    (iff (bounded-nat-listp (append a b) bound)
+         (and (bounded-nat-listp a bound)
+              (bounded-nat-listp b bound))))
+
+  (defthm bounded-nat-listp-of-nil
+    (bounded-nat-listp nil bound))
+
+  (defthm bounded-nat-listp-of-cons
+    (iff (bounded-nat-listp (cons a b) bound)
+         (and (bounded-natp a bound)
+              (bounded-nat-listp b bound)))))
+
+(local
+ (define bounded-nat-listp-badguy (x bound)
+   :verify-guards nil
+   (if (atom x)
+       nil
+     (if (bounded-natp (car x) bound)
+         (bounded-nat-listp-badguy (cdr x) bound)
+       (car x)))
+   ///
+   (defthm bounded-nat-listp-badguy-is-bad
+     (not (bounded-natp (bounded-nat-listp-badguy x bound) bound)))
+
+   (defthmd bounded-nat-listp-when-nat-listp-badguy-not-member
+     (implies (acl2::rewriting-positive-literal `(bounded-nat-listp ,x ,bound))
+              (iff (bounded-nat-listp x bound)
+                   (not (member (bounded-nat-listp-badguy x bound) x))))
+     :hints(("Goal" :in-theory (enable bounded-nat-listp))))
+
+   (defcong set-equiv equal (bounded-nat-listp x bound) 1
+     :hints(("Goal" :in-theory (enable bounded-nat-listp-when-nat-listp-badguy-not-member)
+             :cases ((bounded-nat-listp x bound))
+             :use ((:instance not-bounded-nat-listp-by-member
+                    (x acl2::x-equiv) (k (bounded-nat-listp-badguy x bound)))
+                   (:instance not-bounded-nat-listp-by-member
+                    (x x) (k (bounded-nat-listp-badguy acl2::x-equiv bound)))))))))
+
+(define aig-p (x (var-bound natp))
   (cond ((atom x) (or (booleanp x) ;; const
-                      (natp x))) ;; var
-        ((eq (cdr x) 'nil) (aig-p (car x)))
+                      (bounded-natp x var-bound))) ;; var
+        ((eq (cdr x) 'nil) (aig-p (car x) var-bound))
         ;; this is weird because (nil . nil) is a valid aig but it makes it so 
         ;; nat-listp-aig-vars-when-aig-p holds
         ((eq (car x) 'nil) nil)
-        (t (and (aig-p (car x))
-                (aig-p (cdr x)))))
+        (t (and (aig-p (car x) var-bound)
+                (aig-p (cdr x) var-bound))))
   ///
-  (defthm nat-listp-aig-vars-when-aig-p
-    (iff (nat-listp (acl2::aig-vars x))
-         (aig-p x))
+  (local (defthm aig-p-is-bounded-nat-listp-aig-vars
+           (iff (aig-p x var-bound)
+                (bounded-nat-listp (acl2::aig-vars x) var-bound))))
+
+  (defthm bounded-nat-listp-aig-vars-when-aig-p
+    (iff (bounded-nat-listp (acl2::aig-vars x) var-bound)
+         (aig-p x var-bound))
     :hints(("Goal" :in-theory (enable acl2::aig-atom-p))))
+  (local (in-theory (disable bounded-nat-listp-aig-vars-when-aig-p)))
 
-  (local (defthm aig-p-is-nat-listp-aig-vars
-           (iff (aig-p x)
-                (nat-listp (acl2::aig-vars x)))))
-  (local (in-theory (disable nat-listp-aig-vars-when-aig-p)))
+  (defthm aig-p-when-lesser-bound
+    (implies (and (aig-p x bound1)
+                  (<= (nfix bound1) (nfix bound)))
+             (aig-p x bound)))
 
-  (local (defun nat-listp-badguy (x)
-           (if (atom x)
-               nil
-             (if (natp (car x))
-                 (nat-listp-badguy (cdr x))
-               (car x)))))
-
-  (local (defthm nat-listp-when-nat-listp-badguy-not-member
-           (implies (and (not (member (nat-listp-badguy x) x))
-                         (true-listp x))
-                    (nat-listp x))))
-
-  (local (defthm not-natp-of-nat-listp-badguy
-           (not (natp (nat-listp-badguy x)))
-           :rule-classes :type-prescription))
-
-  (local (defthm nat-listp-implies-not-member-of-non-nat
-           (implies (and (nat-listp x)
-                         (not (natp k)))
-                    (not (member k x)))))
 
   (local (defthm member-aig-vars-aig-and
            (implies (and (not (member v (acl2::aig-vars x)))
@@ -90,71 +158,84 @@
                                     (acl2::member-aig-vars-aig-and))))))
 
   (defthm aig-p-of-aig-not
-    (implies (aig-p x)
-             (aig-p (acl2::aig-not x))))
+    (implies (aig-p x bound)
+             (aig-p (acl2::aig-not x) bound)))
+
+  (local (in-theory (enable bounded-nat-listp-when-nat-listp-badguy-not-member
+                            bounded-nat-listp-implies-not-member)))
 
   (defthm aig-p-of-aig-and
-    (implies (and (aig-p x) (aig-p y))
-             (aig-p (acl2::aig-and x y))))
+    (implies (and (aig-p x bound) (aig-p y bound))
+             (aig-p (acl2::aig-and x y) bound)))
 
-  (local (in-theory (disable aig-p-is-nat-listp-aig-vars)))
+  (local (in-theory (disable aig-p-is-bounded-nat-listp-aig-vars)))
 
   (defthm aig-p-of-aig-or
-    (implies (and (aig-p x) (aig-p y))
-             (aig-p (acl2::aig-or x y)))
+    (implies (and (aig-p x bound) (aig-p y bound))
+             (aig-p (acl2::aig-or x y) bound))
     :hints(("Goal" :in-theory (enable acl2::aig-or))))
 
   (defthm aig-p-of-aig-xor
-    (implies (and (aig-p x) (aig-p y))
-             (aig-p (acl2::aig-xor x y)))
+    (implies (and (aig-p x bound) (aig-p y bound))
+             (aig-p (acl2::aig-xor x y) bound))
     :hints(("Goal" :in-theory (enable acl2::aig-xor))))
 
   (defthm aig-p-of-aig-iff
-    (implies (and (aig-p x) (aig-p y))
-             (aig-p (acl2::aig-iff x y)))
+    (implies (and (aig-p x bound) (aig-p y bound))
+             (aig-p (acl2::aig-iff x y) bound))
     :hints(("Goal" :in-theory (enable acl2::aig-iff))))
 
   (defthm aig-p-of-aig-ite
-    (implies (and (aig-p x) (aig-p y) (aig-p z))
-             (aig-p (acl2::aig-ite x y z)))
+    (implies (and (aig-p x bound) (aig-p y bound) (aig-p z bound))
+             (aig-p (acl2::aig-ite x y z) bound))
     :hints(("Goal" :in-theory (enable acl2::aig-ite))))
 
   (defthm aig-p-of-car
-    (implies (aig-p x)
-             (aig-p (car x))))
+    (implies (aig-p x bound)
+             (aig-p (car x) bound)))
 
   (defthm aig-p-of-cdr
-    (implies (aig-p x)
-             (aig-p (cdr x))))
+    (implies (aig-p x bound)
+             (aig-p (cdr x) bound)))
 
   (defthm aig-atom-p-when-aig-p
-    (implies (aig-p x)
+    (implies (aig-p x bound)
              (equal (acl2::aig-atom-p x)
-                    (atom x)))))
+                    (atom x))))
+  (defthm aig-p-of-var
+    (implies (natp x)
+             (equal (aig-p x var-bound)
+                    (< x (nfix var-bound))))
+    :hints(("Goal" :in-theory (enable bounded-natp)))))
 
-(define aig-fix ((x aig-p))
-  :returns (new-x aig-p :hints(("Goal" :in-theory (enable aig-p))))
+(define aig-fix ((x (aig-p x var-bound)) (var-bound natp))
+  :returns (new-x (aig-p new-x var-bound) :hints(("Goal" :in-theory (enable aig-p))))
   :verify-guards nil
   (mbe :logic (cond ((atom x) (and (or (booleanp x)
-                                       (natp x))
+                                       (bounded-natp x var-bound))
                                    x))
                     ((eq (cdr x) nil)
-                     (cons (aig-fix (car x)) nil))
+                     (cons (aig-fix (car x) var-bound) nil))
                     ((eq (car x) nil) nil)
-                    (t (b* ((car (aig-fix (car x)))
-                            (cdr (aig-fix (cdr x))))
+                    (t (b* ((car (aig-fix (car x) var-bound))
+                            (cdr (aig-fix (cdr x) var-bound)))
                          (and car cdr (cons car cdr)))))
        :exec x)
   ///
   (defthm aig-fix-when-aig-p
-    (implies (aig-p x)
-             (equal (aig-fix x) x))
+    (implies (aig-p x bound)
+             (equal (aig-fix x bound) x))
     :hints(("Goal" :in-theory (enable aig-p))))
 
-  (verify-guards aig-fix :hints(("Goal" :in-theory (enable aig-p))))
-  (fty::deffixtype aig :pred aig-p :fix aig-fix :equiv aig-equiv :define t))
+  (verify-guards aig-fix :hints(("Goal" :in-theory (enable aig-p)))))
 
-(fty::deflist aig-list :pred aig-listp :fix aig-list-fix :elt-type aig :true-listp t)       
+
+
+;; (define aig-listp (x (var-bound natp))
+;;   (if (atom x)
+;;       (eq x nil)
+;;     (and (aig-p (car x) var-bound)
+;;          (aig-listp (cdr x) var-bound))))
         
 
 
